security/BacktranslationProof2.v
@@ -64,25 +64,292 @@ End GENPROOFS.
 (*   (forall (id : ident) (b : block), Genv.find_symbol ge id = Some b -> Plt b thr) -> *)
 (*   forall (gl : list (ident * globdef F V)) (m m' : mem), Genv.alloc_globals ge m gl = Some m' -> Mem.inject_neutral thr m -> Ple (Mem.nextblock m') thr -> Mem.inject_neutral thr m' *)
 
+Section PROOFGENV.
+
+  Lemma gen_prog_defs_props_1
+        (a_ge: Senv.t) tr (gds: list (ident * globdef Asm.fundef unit))
+        (gen_gds1: list (ident * globdef Clight.fundef type))
+        cnts params
+        (GEN: gen_gds1 = (map (fun '(id, gd) => (id, gen_progdef a_ge (get_id_tr tr id) gd (cnts ! id) (params ! id))) gds))
+    :
+    Forall (fun '(id, gd_c) =>
+              exists gd_a, (In (id, gd_a) gds) /\ (gd_c = gen_progdef a_ge (get_id_tr tr id) gd_a (cnts ! id) (params ! id)))
+           gen_gds1.
+  Proof.
+    subst gen_gds1. rewrite Forall_map. apply Forall_forall. i. des_ifs. esplits; eauto.
+  Qed.
+
+  Lemma gen_prog_defs_inv_1
+        (a_ge: Senv.t) tr (gds: list (ident * globdef Asm.fundef unit))
+        (gen_gds1: list (ident * globdef Clight.fundef type))
+        cnts params
+        (GEN: gen_gds1 = (map (fun '(id, gd) => (id, gen_progdef a_ge (get_id_tr tr id) gd (cnts ! id) (params ! id))) gds))
+        id gd
+        (IN: In (id, gd) gds)
+    :
+    In (id, gen_progdef a_ge (get_id_tr tr id) gd (cnts ! id) (params ! id)) gen_gds1.
+  Proof.
+    eapply (in_map (fun '(id0, gd0) => (id0, gen_progdef a_ge (get_id_tr tr id0) gd0 cnts ! id0 params ! id0))) in IN. clarify.
+  Qed.
+
+  Lemma gen_counter_defs_props
+        (gds: list (ident * globdef Asm.fundef unit))
+        cnts x0
+        (CNTS: cnts = gen_counter_defs x0 gds)
+    :
+    Forall (fun '(id, (cnt, gd_c)) =>
+              (cnt = (id + x0)%positive) /\ (exists gd_a, (In (id, gd_a) gds) /\ (gd_c = gen_counter (comp_of gd_a))))
+           (PTree.elements cnts).
+  Proof.
+    subst. rewrite Forall_forall. i. destruct x as (id & (cnt & gd_c)). unfold gen_counter_defs in H.
+    apply PTree.elements_complete in H. apply PTree_Properties.in_of_list in H.
+    apply list_in_map_inv in H. des. des_ifs. splits; auto. esplits; eauto.
+  Qed.
+
+  Lemma gen_counter_defs_inv
+        (gds: list (ident * globdef Asm.fundef unit))
+        (NR: list_norepet (map fst gds))
+        cnts x0
+        (CNTS: cnts = gen_counter_defs x0 gds)
+        id gd
+        (IN: In (id, gd) gds)
+    :
+    cnts ! id = Some ((id + x0)%positive, gen_counter (comp_of gd)).
+    (* In (id, ((id + x0)%positive, gen_counter (comp_of gd))) (PTree.elements cnts). *)
+  Proof.
+    subst. unfold gen_counter_defs. apply PTree_Properties.of_list_norepet.
+    { rewrite map_map.
+      match goal with
+      | [|- list_norepet (map ?f gds)] => assert (f = fst)
+      end.
+      { extensionalities s. des_ifs. }
+      rewrite H. auto.
+    }
+    { eapply (in_map (fun '(id0, gd0) => (id0, ((id0 + x0)%positive, gen_counter (comp_of gd0))))) in IN. auto. }
+  Qed.
+
+
+
+wf_counters = 
+fun (ge : genv) (m : mem) (tr : bundle_trace) (cnts : cnt_ids) =>
+(forall (id0 id1 : positive) (cnt : ident),
+ cnts ! id0 = Some cnt -> cnts ! id1 = Some cnt -> id0 = id1) /\
+(forall (id : ident) (b : block) (f : function),
+ Genv.find_symbol ge id = Some b ->
+ Genv.find_funct_ptr ge b = Some (Internal f) ->
+ exists cnt : ident,
+   cnts ! id = Some cnt /\
+   wf_counter ge m (comp_of f) (Datatypes.length (get_id_tr tr id)) cnt)
+     : genv -> mem -> bundle_trace -> cnt_ids -> Prop
+  
+Forall_map: forall [A B : Type] (f : A -> B) (P : B -> Prop) (l : list A), Forall P (map f l) <-> Forall (fun x : A => P (f x)) l
+Forall_image:
+  forall [A B : Type] (f : A -> B) (l : list B),
+  Forall (fun y : B => exists x : A, y = f x) l <-> (exists l' : list A, l = map f l')
+
+  Lemma gen_prog_defs_props
+        (a_ge: Senv.t) tr (gds: list (ident * globdef Asm.fundef unit))
+        (gen_gds: list (ident * globdef Clight.fundef type))
+        cnts params
+        (GEN: gen_gds = (map (fun '(id, gd) => (id, gen_progdef a_ge (get_id_tr tr id) gd (cnts ! id) (params ! id))) gds) ++ cnt_defs)
+    :
+    Forall (fun '(id, gd_c) =>
+              ((id < r_cnt) ->
+               exists gd_a, (In (id, gd_a) gds) /\ (gd_c = gen_progdef a_ge (get_id_tr tr id) gd_a (cnts ! id) (params ! id))) /\
+                (r_cnt <= id
+    
+    
+        
+        
+
+  (* Lemma gen_program_genv *)
+  (*       btr (p_a: Asm.program) (p_c: Clight.program) *)
+  (*       (P_C: p_c = gen_program btr p_a) *)
+  (*   : *)
+    
+
+    
+  Definition gen_prog_defs (a_ge: Senv.t) tr (gds: list (ident * globdef Asm.fundef unit)): list (ident * globdef Clight.fundef type) :=
+    let m0 := next_id gds in
+    let cnts := gen_counter_defs m0 gds in
+    let cnt_defs := map snd (PTree.elements cnts) in
+    let m1 := next_id cnt_defs in
+    let params := gen_params m1 gds in
+    (map (fun '(id, gd) => (id, gen_progdef a_ge (get_id_tr tr id) gd (cnts ! id) (params ! id))) gds) ++ cnt_defs.
+
+
+Genv.find_symbol_exists:
+  forall [F V : Type] (p : AST.program F V) (id : ident) (g : globdef F V),
+  In (id, g) (AST.prog_defs p) -> exists b : block, Genv.find_symbol (Genv.globalenv p) id = Some b
+Genv.find_symbol_inversion:
+  forall [F V : Type] (p : AST.program F V) (x : ident) [b : block],
+  Genv.find_symbol (Genv.globalenv p) x = Some b -> In x (prog_defs_names p)
+
+
+Genv.globalenv = 
+fun (F V : Type) (p : AST.program F V) =>
+Genv.add_globals (Genv.empty_genv F V (AST.prog_public p) (AST.prog_pol p)) (AST.prog_defs p)
+     : forall F V : Type, AST.program F V -> Genv.t F V
+
+End PROOFGENV.
+
 
 Section PROOFINIT.
+
+  Lemma gen_counter_defs_alloc
+        x0 gds cnts
+        (CNTS: cnts = gen_counter_defs x0 gds)
+        (ge: genv)
+    :
+    Forall (fun (idg: ident * (globdef fundef type)) =>
+              let (_, y) := idg in
+              match y with
+              | Gfun _ => False
+              | Gvar v =>
+                  Genv.init_data_list_aligned 0 (gvar_init v) /\
+                    (forall (i : ident) (o : ptrofs), In (Init_addrof i o) (gvar_init v) -> exists b : block, Genv.find_symbol ge i = Some b)
+              end) (map snd (PTree.elements cnts)).
+  Proof.
+    
+                  
+    let cnts := gen_counter_defs m0 gds in
+    let cnt_defs := map snd (PTree.elements cnts) in
+wf_counter = 
+fun (ge : Senv.t) (m : mem) (cp : compartment) (n : nat) (cnt : ident) =>
+Senv.public_symbol ge cnt = false /\
+(exists b : block,
+   Senv.find_symbol ge cnt = Some b /\
+   Mem.valid_access m Mint64 b 0 Writable (Some cp) /\ Mem.loadv Mint64 m (Vptr b Ptrofs.zero) (Some cp) = Some (Vlong (nat64 n)))
+     : Senv.t -> mem -> compartment -> nat -> ident -> Prop
+
+gen_counter_defs = 
+fun (m : positive) (gds : list (ident * globdef Asm.fundef unit)) =>
+fold_left
+  (fun (pt : PTree.tree (positive * globdef fundef type)) '(id, gd) => PTree.set id ((id + m)%positive, gen_counter (comp_of gd)) pt)
+  gds (PTree.empty (positive * globdef fundef type))
+     : positive -> list (ident * globdef Asm.fundef unit) -> PTree.t (ident * globdef fundef type)
+
+Genv.alloc_global_exists:
+  forall [F V : Type] {CF : has_comp F} (ge : Genv.t F V) (m : mem) (idg : ident * globdef F V),
+  (let (_, y) := idg in
+   match y with
+   | Gfun _ => True
+   | Gvar v =>
+       Genv.init_data_list_aligned 0 (gvar_init v) /\
+       (forall (i : ident) (o : ptrofs), In (Init_addrof i o) (gvar_init v) -> exists b : block, Genv.find_symbol ge i = Some b)
+   end) -> exists m' : mem, Genv.alloc_global ge m idg = Some m'
+
+
+Genv.alloc_globals = 
+fun (F V : Type) (CF : has_comp F) (ge : Genv.t F V) =>
+fix alloc_globals (m : mem) (gl : list (ident * globdef F V)) {struct gl} : option mem :=
+  match gl with
+  | [] => Some m
+  | g :: gl' => match Genv.alloc_global ge m g with
+                | Some m' => alloc_globals m' gl'
+                | None => None
+                end
+  end
+      : forall F V : Type, has_comp F -> Genv.t F V -> mem -> list (ident * globdef F V) -> option mem
+
+Genv.alloc_globals_app:
+  forall [F V : Type] {CF : has_comp F} (ge : Genv.t F V) (gl1 gl2 : list (ident * globdef F V)) (m : mem) [m1 : mem],
+  Genv.alloc_globals ge m gl1 = Some m1 -> Genv.alloc_globals ge m1 gl2 = Genv.alloc_globals ge m (gl1 ++ gl2)
+
+Genv.init_mem = 
+fun (F V : Type) (CF : has_comp F) (p : AST.program F V) => Genv.alloc_globals (Genv.globalenv p) Mem.empty (AST.prog_defs p)
+     : forall F V : Type, has_comp F -> AST.program F V -> option mem
+
+Genv.globals_initialized = 
+fun (F V : Type) (ge g : Genv.t F V) (m : mem) =>
+forall (b : block) (gd : globdef F V),
+Genv.find_def g b = Some gd ->
+match gd with
+| Gfun _ =>
+    Mem.perm m b 0 Cur Nonempty /\
+    (forall (ofs : Z) (k : perm_kind) (p : permission), Mem.perm m b ofs k p -> ofs = 0 /\ p = Nonempty)
+| Gvar v =>
+    Mem.range_perm m b 0 (init_data_list_size (gvar_init v)) Cur (Genv.perm_globvar v) /\
+    (forall (ofs : Z) (k : perm_kind) (p : permission),
+     Mem.perm m b ofs k p -> 0 <= ofs < init_data_list_size (gvar_init v) /\ perm_order (Genv.perm_globvar v) p) /\
+    (gvar_volatile v = false -> Genv.load_store_init_data ge m b 0 (gvar_init v) (Some (gvar_comp v))) /\
+    (gvar_volatile v = false ->
+     Mem.loadbytes m b 0 (init_data_list_size (gvar_init v)) (Some (gvar_comp v)) =
+     Some (Genv.bytes_of_init_data_list ge (gvar_init v)))
+end
+     : forall F V : Type, Genv.t F V -> Genv.t F V -> mem -> Prop
+  Lemma c_exists_init_mem
+        btr (p: Asm.program)
+        m_a
+        (MEMA: Genv.init_mem p = Some m_a)
+    :
+    exists m_c, Genv.init_mem (gen_program btr p) = Some m_c.
+
+
+
+  Definition gen_prog_defs (a_ge: Senv.t) tr (gds: list (ident * globdef Asm.fundef unit)): list (ident * globdef Clight.fundef type) :=
+    let m0 := next_id gds in
+    let cnts := gen_counter_defs m0 gds in
+    let cnt_defs := map snd (PTree.elements cnts) in
+    let m1 := next_id cnt_defs in
+    let params := gen_params m1 gds in
+    (map (fun '(id, gd) => (id, gen_progdef a_ge (get_id_tr tr id) gd (cnts ! id) (params ! id))) gds) ++ cnt_defs.
+
+  Program Definition gen_program tr (a_p: Asm.program): Clight.program :=
+    let a_ge := Genv.globalenv a_p in
+    @Build_program _
+                   (gen_prog_defs a_ge tr a_p.(AST.prog_defs))
+                   (AST.prog_public a_p)
+                   (AST.prog_main a_p)
+                   (AST.prog_pol a_p)
+                   []
+                   (@PTree.empty composite)
+                   _.
+
+
+
+
+
+Variant ir_initial_state (p : Asm.program) : ir_state -> Prop :=
+    ir_initial_state_intro : forall (cur : block) (m0 : mem),
+                             let ge := Genv.globalenv p in
+                             Genv.find_symbol ge (AST.prog_main p) = Some cur ->
+                             (exists f : Asm.function, Genv.find_funct_ptr ge cur = Some (AST.Internal f)) ->
+                             Genv.init_mem p = Some m0 -> ir_initial_state p (Some (cur, m0, [])).
+Inductive initial_state (p: program): state -> Prop :=
+  | initial_state_intro: forall b f m0,
+      let ge := Genv.globalenv p in
+      Genv.init_mem p = Some m0 ->
+      Genv.find_symbol ge p.(prog_main) = Some b ->
+      Genv.find_funct_ptr ge b = Some f ->
+      type_of_fundef f = Tfunction Tnil type_int32s cc_default ->
+      initial_state p (Callstate f nil Kstop m0).
+  Definition wf_c_state (ge: Clight.genv) (tr ttr: bundle_trace) (cnts: cnt_ids) id (cst: Clight.state) :=
+    match cst with
+    | State f stmt k_c e le m_c =>
+        wf_counters ge m_c tr cnts /\
+          (exists m_c', Mem.free_list m_c (blocks_of_env ge e) (comp_of f) = Some m_c' /\ wf_c_cont ge m_c' k_c) /\
+          wf_c_stmt ge (comp_of f) cnts id ttr stmt /\
+          (wf_env ge e /\ (not_global_blks (ge) (blocks_of_env2 ge e)) /\ (wf_c_nb ge m_c))
+    | _ => False
+    end.
+  Definition match_state (ge_i: Asm.genv) (ge_c: Clight.genv) (k: meminj) tr cnts pars id (ist: ir_state) (cst: Clight.state) :=
+    match ist, cst with
+    | Some (cur, m_i, k_i), State f _ k_c e le m_c =>
+        (match_genv ge_i ge_c) /\ (match_mem ge_i k m_i m_c) /\
+          (match_cur_fun ge_i ge_c cur f id) /\ (match_find_def ge_i ge_c cnts pars tr) /\
+          (match_cont ge_c tr cnts k_c k_i) /\
+          (match_params pars ge_c ge_i) /\
+          (match_cnts cnts ge_c k)
+    | _, _ => False
+    end.
+
+
 
   Definition asm_program_does_prefix (p: Asm.program) (t: trace) :=
     semantics_has_initial_trace_prefix (Asm.semantics p) t.
   Definition clight_program_does_prefix (p: Clight.program) (t: trace) :=
     semantics_has_initial_trace_prefix (Clight.semantics1 p) t.
-
-  (* Lemma behaves_star_prefix *)
-  (*       L beh *)
-  (*       (s: Smallstep.state L) *)
-  (*       (BEH: state_behaves L s beh) *)
-  (*       tr *)
-  (*       (PRE: behavior_prefix tr beh) *)
-  (*   : *)
-  (*   exists s', Star L s tr s'. *)
-  (* Proof. *)
-
-  (* Admitted. *)
 
   Theorem asm_to_clight
           (p: Asm.program) (ast: Asm.state)
@@ -112,7 +379,24 @@ Section PROOFINIT.
     }
     { eapply MS_I. }
     intros (btr & ist' & UTR & ISTAR). esplits. 2: eauto.
-    eapply semantics_has_initial_trace_cut_implies_prefix. econs 1; ss.
+    eapply semantics_has_initial_trace_cut_implies_prefix.
+    assert (INIT_C: exists cst, Clight.initial_state (gen_program btr p) cst).
+    { admit. }
+    des. hexploit ir_to_clight.
+    { eapply wf_program_wf_ge; eauto. }
+    4: eapply ISTAR.
+    { admit. }
+    { admit. }
+    { admit. }
+    intros CSTAR. des. econs 1; ss.
+    { admit. }
+    hexploit state_behaves_exists. intros (beh2 & BEH2).
+    esplits.
+    { admit. }
+    { eapply BEH2. }
+
+  Admitted.
+  Qed.
 
     TODO
 
